ipow: use absint

bedrock2/src/Examples/ipow.v
@@ -9,49 +9,73 @@ Local Coercion var (x : string) : Syntax.expr := Syntax.expr.var x.
 Definition ipow := ("ipow", (["x";"e"], (["ret"]:list varname), bedrock_func_body:(
   "ret" = 1;;
   while ("e") {{
-    "t" = "e" .& 1;;
-    if ("t") {{ "ret" = "ret" * "x" }};;
+    if ("e" .& 1) {{ "ret" = "ret" * "x" }};;
     "e" = "e" >> 1;;
-    "x" = "x" * "x";;
-    Syntax.cmd.unset "t"
+    "x" = "x" * "x"
   }}
 ))).
 
-Require Import Coq.micromega.Lia.
-Local Ltac mia := Z.div_mod_to_equations; nia.
-
-Require Import bedrock2.BasicC64Semantics coqutil.Word.Interface.
-Require bedrock2.WeakestPrecondition coqutil.Word.Properties.
+From bedrock2 Require Import Semantics BasicC64Semantics WeakestPrecondition ProgramLogic.
+From coqutil Require Import Word.Properties Word.Interface Tactics.letexists.
 
 Definition spec_of_ipow := fun functions =>
   forall x e t m,
     WeakestPrecondition.call functions
       "ipow" t m [x; e]
       (fun t' m' rets => t=t'/\ m=m' /\ exists v, rets = [v] /\ (
-        word.unsigned x ^ word.unsigned e < 2^64 ->
-        word.unsigned v = word.unsigned x ^ word.unsigned e)).
+        word.unsigned v = word.unsigned x ^ word.unsigned e mod 2^width)).
 
-From coqutil.Tactics Require Import letexists eabstract.
-Require Import bedrock2.ProgramLogic.
-Require Import AdmitAxiom.
+
+Module Z.
+  Lemma pow_mod x n m (Hnz: m <> 0) : (x mod m)^n mod m = x^n mod m.
+  Proof.
+    revert n.
+    eapply Z.order_induction_0; intros.
+    { intros ???; subst; split; auto. }
+    { rewrite 2Z.pow_0_r; trivial. }
+    { rewrite 2Z.pow_succ_r by trivial.
+      rewrite <-Z.mul_mod_idemp_r by trivial.
+      multimatch goal with H: _ |- _ => rewrite H end;
+      rewrite Z.mul_mod_idemp_l, Z.mul_mod_idemp_r; solve[trivial]. }
+    { rewrite 2Z.pow_neg_r; trivial. }
+  Qed.
+  
+  Lemma mod2_nonzero x : x mod 2 <> 0 -> x mod 2 = 1.
+  Proof. Z.div_mod_to_equations. Lia.lia. Qed.
+
+  Lemma land_1_r x : Z.land x 1 = x mod 2.
+  Proof.
+    change 1 with (Z.ones 1) in *.
+    rewrite Z.land_ones in * by discriminate.
+    exact eq_refl.
+  Qed.
+End Z.
+
+Require Import bedrock2.TODO_absint Coq.micromega.Lia.
+
+Ltac t :=
+  repeat match goal with x := _ |- _ => subst x end;
+  repeat match goal with |- context [word.unsigned ?e] => progress (idtac; let H := rbounded (word.unsigned e) in idtac) end;
+  repeat match goal with G: context [word.unsigned ?e] |- _ => progress (idtac; let H := rbounded (word.unsigned e) in idtac) end;
+  repeat match goal with |- context [word.unsigned ?e] => progress (idtac; let H := unsigned.zify_expr e in try rewrite H) end;
+  repeat match goal with G: context [word.unsigned ?e] |- _ => progress (idtac; let H := unsigned.zify_expr e in try rewrite H in G) end;
+  repeat match goal with H: unsigned.absint_eq ?x ?x |- _ => clear H end;
+  cbv [unsigned.absint_eq] in *.
+
 Lemma ipow_ok : forall functions, spec_of_ipow (ipow::functions).
 Proof.
-  bind_body_of_function ipow; cbv [spec_of_ipow].
-  intros.
-  hnf. (* incoming call dispatch *)
-  letexists. split; [exact eq_refl|]. (* argument initialization *)
-
+  bind_body_of_function ipow; cbv [spec_of_ipow]; intros; hnf.
   repeat straightline.
 
-  Import Word.Properties.word Word.Interface.word.
-  refine (TailRecursion.tailrec HList.polymorphic_list.nil (["e";"ret";"x"] : list varname)
-    (fun v t m e ret x => PrimitivePair.pair.mk (v = word.unsigned e)
-    (fun t' m' e' ret' x' => t' = t /\ m' = m /\
-       (unsigned ret * unsigned x ^ unsigned e < 2^64 ->
-        unsigned ret' = unsigned ret * unsigned x ^ unsigned e)))
-    (fun n m => 0 <= n < m)
+  refine (TailRecursion.tailrec
+    (* types of ghost variables*) HList.polymorphic_list.nil
+    (* program variables *) ["e";"ret";"x"]
+    (fun v t m e ret x => PrimitivePair.pair.mk (v = word.unsigned e) (* precondition *)
+    (fun   T M E RET X => T = t /\ M = m /\ (* postcondition *)
+        word.unsigned RET = word.unsigned ret * word.unsigned x ^ word.unsigned e mod 2^width))
+    (fun n m => 0 <= n < m) (* well_founded relation *)
     _ _ _ _ _);
-
+    (* TODO wrap this into a tactic with the previous refine *)
     cbn [HList.hlist.foralls HList.tuple.foralls
          HList.hlist.existss HList.tuple.existss
          HList.hlist.apply  HList.tuple.apply
@@ -66,122 +90,45 @@ Proof.
   { (* loop test *)
     repeat straightline; try show_program.
     { (* loop body *)
-      letexists; split; [eabstract (repeat straightline)|]. (* if condition *)
+      letexists; split; [repeat straightline|]. (* if condition evaluation *)
       split. (* if cases, path-blasting *)
-      { repeat straightline.
+      { repeat (straightline || (split; trivial; [])); t.
         { (* measure decreases *)
-          cbn [parameters Semantics.interp_binop Semantics.width] in *.
-          pose proof (unsigned_range x0) as pf.
-          repeat match goal with
-                   |- context [?x] => subst x
-                 end.
-          rewrite ?unsigned_sru_nowrap,
-                  ?unsigned_of_Z,
-                  ?Z.shiftr_div_pow2
-            by (cbv; congruence).
-          change Semantics.width with 64 in *.
-          change (2 ^ (1 mod 2 ^ 64)) with 2.
-          mia. }
+          set (word.unsigned x0) in *. (* WHY does lia need this? *)
+          Z.div_mod_to_equations; Lia.lia. }
         { (* invariant preserved *)
-          repeat split; try exact eq_refl; intros.
-          cbn [parameters Semantics.interp_binop Semantics.width] in *.
-          replace (unsigned x0) with (2 * (unsigned x0 / 2) + 1) in * by (subst v1; revert H0; admit).
-          rewrite ?Z.pow_add_r, Z.pow_twice_r, ?Z.pow_1_r, ?Z.pow_mul_l, ?Z.mul_assoc in * by ((intro;discriminate)||admit).
-          rewrite H3; cycle 1;
-            repeat match goal with
-                     |- context [?x] => subst x
-                   end;
-            repeat rewrite ?unsigned_of_Z,
-                           ?unsigned_sru_nowrap,
-                           ?unsigned_mul,
-                           ?Z.mul_mod_idemp_l,
-                           ?Z.shiftr_div_pow2;
-            change Semantics.width with 64 in *;
-            change (1 mod 2 ^ 64) with 1; change (2^1) with 2; try Lia.lia.
-          { rewrite !Z.mod_small by (revert H1; admit). rewrite Z.pow_mul_l. abstract mia. }
-          { rewrite !Z.mod_small by (revert H1; admit). rewrite Z.pow_mul_l. abstract ring. } } }
-      {
-        straightline; [].
-        straightline; [].
-        straightline; [].
-        (* repeat straightline. *)
-        (* Error: Anomaly "Universe Top.196 undefined." Please report at http://coq.inria.fr/bugs/. *)
-        straightline; [].
-        repeat straightline.
+          rewrite H3; clear H3. rename H0 into Hbit.
+          erewrite Z.land_1_r in *; change (2^1) with 2 in *.
+          eapply Z.mod2_nonzero in Hbit.
+          epose proof (Z.div_mod _ 2 ltac:(discriminate)) as Heq; rewrite Hbit in Heq.
+          rewrite Heq at 2; clear Hbit Heq.
+          (* rewriting with equivalence modulo ... *)
+          rewrite !word.unsigned_mul, ?Z.mul_mod_idemp_l by discriminate.
+          rewrite <-(Z.mul_mod_idemp_r _ (_^_)), Z.pow_mod by discriminate.
+          rewrite ?Z.pow_add_r by (pose proof word.unsigned_range x0; Z.div_mod_to_equations; Lia.lia).
+          rewrite ?Z.pow_twice_r, ?Z.pow_1_r, ?Z.pow_mul_l.
+          rewrite Z.mul_mod_idemp_r by discriminate.
+          f_equal; ring. } }
+      { repeat (straightline || (split; trivial; [])); t.
         { (* measure decreases *)
-          cbn [parameters Semantics.interp_binop Semantics.width] in *.
-          pose proof (unsigned_range x0) as pf.
-          repeat match goal with
-                   |- context [?x] => subst x
-                 end.
-          rewrite ?unsigned_sru_nowrap,
-                  ?unsigned_of_Z,
-                  ?Z.shiftr_div_pow2
-            by (cbv; congruence).
-            change Semantics.width with 64 in *;
-          change (2 ^ (1 mod 2 ^ 64)) with 2.
-          mia. }
+          set (word.unsigned x0) in *. (* WHY does lia need this? *)
+          Z.div_mod_to_equations; Lia.lia. }
         { (* invariant preserved *)
-          repeat split; try exact eq_refl; intros.
-          cbn [parameters Semantics.interp_binop Semantics.width] in *.
-          replace (unsigned x0) with (2 * (unsigned x0 / 2)) in * by (subst v1; revert H0; admit).
-          rewrite ?Z.pow_add_r, Z.pow_twice_r, ?Z.pow_1_r, ?Z.pow_mul_l, ?Z.mul_assoc in *.
-          rewrite H3; cycle 1;
-            repeat match goal with
-                     |- context [?x] => subst x
-                   end;
-            repeat rewrite ?word.unsigned_of_Z,
-                           ?unsigned_sru_nowrap,
-                           ?unsigned_mul,
-                           ?Z.mul_mod_idemp_l,
-                           ?Z.shiftr_div_pow2;
-            change Semantics.width with 64 in *;
-            change (1 mod 2 ^ 64) with 1; change (2^1) with 2; try Lia.lia.
-          { rewrite !Z.mod_small by (revert H1; admit). rewrite Z.pow_mul_l. abstract mia. }
-          { rewrite !Z.mod_small by (revert H1; admit). rewrite Z.pow_mul_l. abstract ring. } } } }
-    { (* end of loop *)
-      repeat split; intros.
-      replace (unsigned x0) with 0 in * by (revert H; admit).
-      rewrite Z.pow_0_r, Z.mul_1_r. exact eq_refl. } }
+          rewrite H3; clear H3. rename H0 into Hbit.
+          rewrite Z.land_1_r in *; change (2^1) with 2 in *.
+          epose proof (Z.div_mod _ 2 ltac:(discriminate)) as Heq; rewrite Hbit in Heq.
+          rewrite Heq at 2; clear Hbit Heq.
+          (* rewriting with equivalence modulo ... *)
+          rewrite !word.unsigned_mul, ?Z.mul_mod_idemp_l by discriminate.
+          rewrite <-(Z.mul_mod_idemp_r _ (_^_)), Z.pow_mod by discriminate.
+          rewrite ?Z.add_0_r, Z.pow_twice_r, ?Z.pow_1_r, ?Z.pow_mul_l.
+          rewrite Z.mul_mod_idemp_r by discriminate.
+          f_equal; ring. } } }
+    { (* postcondition *) rewrite H, Z.pow_0_r, Z.mul_1_r, word.wrap_unsigned; auto. } }
 
-  (* Error: Anomaly "Universe Top.427 undefined." Please report at http://coq.inria.fr/bugs/. *)
-  straightline; [].
-  straightline; [].
-  straightline; [].
-  straightline; [].
-  straightline; [].
-  straightline; [].
-  straightline; [].
-  straightline; [].
-  straightline; [].
-  straightline; [].
   repeat straightline.
 
-  (* function postcondition *)
-  repeat eapply conj; try exact eq_refl.
-  letexists. split; [exact eq_refl|].
-  intros.
-  repeat match goal with
-           |- context [?x] => subst x
-         end.
-  subst v. rewrite ?unsigned_of_Z, ?Z.mul_1_l in *.
-  rewrite H1; trivial.
-
-  Unshelve. (* WHY does this not get admits? *)
-
-  Grab Existential Variables.
-
-(* 11 subgoals (ID 6265) *)
-(*  word_test x0 = false -> 0 = unsigned x0 *)
-(*  unsigned x1 * unsigned x2 ^ (unsigned x0 / 2) * unsigned x2 ^ (unsigned x0 / 2) < 2 ^ 64 -> 0 <= unsigned x2 * unsigned x2 < 2 ^ 64 *)
-(*  unsigned x1 * unsigned x2 ^ (unsigned x0 / 2) * unsigned x2 ^ (unsigned x0 / 2) < 2 ^ 64 -> 0 <= unsigned x2 * unsigned x2 < 2 ^ 64 *)
-(*  word_test (and x0 (of_Z 1)) = false -> 2 * (unsigned x0 / 2) = unsigned x0 *)
-(*  unsigned x1 * unsigned x2 ^ (unsigned x0 / 2) * unsigned x2 ^ (unsigned x0 / 2) * unsigned x2 < 2 ^ 64 -> 0 <= unsigned x2 * unsigned x2 < 2 ^ 64 *)
-(*  unsigned x1 * unsigned x2 ^ (unsigned x0 / 2) * unsigned x2 ^ (unsigned x0 / 2) * unsigned x2 < 2 ^ 64 -> 0 <= unsigned x1 * unsigned x2 < 2 ^ 64 *)
-(*  unsigned x1 * unsigned x2 ^ (unsigned x0 / 2) * unsigned x2 ^ (unsigned x0 / 2) * unsigned x2 < 2 ^ 64 -> 0 <= unsigned x2 * unsigned x2 < 2 ^ 64 *)
-(*  unsigned x1 * unsigned x2 ^ (unsigned x0 / 2) * unsigned x2 ^ (unsigned x0 / 2) * unsigned x2 < 2 ^ 64 -> 0 <= unsigned x1 * unsigned x2 < 2 ^ 64 *)
-(*  0 <= 2 * (unsigned x0 / 2) *)
-(*  0 <= 2 * (unsigned x0 / 2) *)
-(*  word_test (and x0 (of_Z 1)) = true -> 2 * (unsigned x0 / 2) + 1 = unsigned x0 *)
-
+  (* function postcontition *)
+  repeat (split || letexists || t || trivial).
+  setoid_rewrite H1; setoid_rewrite Z.mul_1_l; trivial.
 Defined.
