bedrock2/src/TODO_absint.v
@@ -1,0 +1,248 @@
+Require Import Coq.Strings.String Coq.ZArith.ZArith.
+From coqutil Require Import Word.Interface Word.Properties.
+From coqutil Require Import Tactics.rdelta Z.div_mod_to_equations.
+
+(* TODO: generalize over word *)
+From bedrock2 Require Import Semantics BasicC64Semantics.
+(** Bounds propagation *)
+
+Lemma Z__range_add a0 a a1 (Ha: a0 <= a < a1) b0 b b1 (Hb : b0 <= b < b1)
+      : a0+b0 <= a+b < a1 + b1 - 1.
+Proof. Lia.nia. Qed.
+Lemma Z__range_sub a0 a a1 (Ha: a0 <= a < a1) b0 b b1 (Hb : b0 <= b < b1)
+      : a0-b1+1 <= a-b < a1 - b0.
+Proof. Lia.nia. Qed.
+Lemma Z__range_div_pos_const_r n0 n n1 (Hn : n0 <= n < n1) d (Hd : 0 < d)
+  : n0/d <= n/d < n1/d + 1.
+Proof. Z.div_mod_to_equations. Lia.nia. Qed.
+Lemma Z__range_mul_nonneg a0 a a1 (Ha: a0 <= a < a1) b0 b b1 (Hb : b0 <= b < b1) (Ha0 : 0 <= a0) (Hb0 : 0 <= b0)
+      : a0*b0 <= a*b < (a1-1)*(b1-1) + 1.
+Proof. Lia.nia. Qed.
+Lemma boundscheck {x0 x x1} (H: x0 <= x < x1) {X0 X1} (Hcheck : andb (X0 <=? x0) (x1 <=? X1) = true) : X0 <= x < X1.
+Proof. eapply andb_prop in Hcheck; case Hcheck; intros H1 H2; eapply Z.leb_le in H1; eapply Z.leb_le in H2. Lia.lia. Qed.
+Lemma boundscheck_lt {x0 x x1} (H: x0 <= x < x1) {X1} (Hcheck: Z.ltb x1 X1 = true) : x < X1.
+Proof. eapply Z.ltb_lt in Hcheck. Lia.lia. Qed.
+Lemma bounded_constant c : c <= c < c+1. Proof. Lia.lia. Qed.
+
+Ltac named_pose_proof pf :=
+  let H := fresh in
+  let __ := match constr:(Set) with _ => pose proof pf as H end in
+  H.
+Ltac named_pose pf :=
+  let H := fresh in
+  let __ := match constr:(Set) with _ => pose pf as H end in
+  H.
+Ltac named_pose_asfresh pf x :=
+  let H := fresh x in
+  let __ := match constr:(Set) with _ => pose pf as H end in
+  H.
+
+Ltac requireZcst z :=
+  lazymatch Coq.setoid_ring.InitialRing.isZcst z with
+  | true => idtac
+  end.
+Ltac requireZcstExpr e :=
+  match e with
+  | Z.pred ?x => requireZcstExpr x
+  | Z.succ ?x => requireZcstExpr x
+  | Z.ones ?x => requireZcstExpr x
+  | Z.opp ?x => requireZcstExpr x
+  | Z.lnot ?x => requireZcstExpr x
+  | Z.add ?x ?y => requireZcstExpr x; requireZcstExpr y
+  | Z.sub ?x ?y => requireZcstExpr x; requireZcstExpr y
+  | Z.mul ?x ?y => requireZcstExpr x; requireZcstExpr y
+  | Z.div ?x ?y => requireZcstExpr x; requireZcstExpr y
+  | Z.modulo ?x ?y => requireZcstExpr x; requireZcstExpr y
+  | Z.quot ?x ?y => requireZcstExpr x; requireZcstExpr y
+  | Z.rem ?x ?y => requireZcstExpr x; requireZcstExpr y
+  | Z.pow ?x ?y => requireZcstExpr x; requireZcstExpr y
+  | Z.shiftl ?x ?y => requireZcstExpr x; requireZcstExpr y
+  | Z.shiftr ?x ?y => requireZcstExpr x; requireZcstExpr y
+  | Z.land ?x ?y => requireZcstExpr x; requireZcstExpr y
+  | Z.lor ?x ?y => requireZcstExpr x; requireZcstExpr y
+  | Z.lxor ?x ?y => requireZcstExpr x; requireZcstExpr y
+  | Z.ldiff ?x ?y => requireZcstExpr x; requireZcstExpr y
+  | Z.clearbit ?x ?y => requireZcstExpr x; requireZcstExpr y
+  | Z.setbit ?x ?y => requireZcstExpr x; requireZcstExpr y
+  | Z.min ?x ?y => requireZcstExpr x; requireZcstExpr y
+  | Z.max ?x ?y => requireZcstExpr x; requireZcstExpr y
+  | Z.gcd ?x ?y => requireZcstExpr x; requireZcstExpr y
+  | Z.lcm ?x ?y => requireZcstExpr x; requireZcstExpr y
+  | _ => requireZcst e
+  end.
+
+Ltac zsimp x :=
+  match constr:(Set) with
+  | _ => let __ := requireZcstExpr x in let y := eval cbv in x in y
+  | _ => x
+  end.
+
+Local Notation "zbsimp! H" :=
+  (ltac:(
+     lazymatch type of H with
+           ?L <= ?X < ?R =>
+           let L := zsimp L in
+           let R := zsimp R in
+           exact ((H : L <= X < R))
+         end
+  )) (at level 10, only parsing).
+
+Ltac rbounded e :=
+  let re := rdelta e in
+  match goal with
+  | H :  _ <= e < _ |- _ => H
+  | _ =>
+    match re with
+    | word.unsigned ?a =>
+      named_pose_proof (zbsimp! (Properties.word.unsigned_range a : _ <= e < _))
+    | Z.div ?a ?b => (* TODO: non-constant denominator? *)
+      let __ := match constr:(Set) with _ => requireZcstExpr b end in
+      let Ha := rbounded a in
+      named_pose_proof (zbsimp! (Z__range_div_pos_const_r _ a _ Ha b ltac:(eapply Z.ltb_lt; exact eq_refl) : _ <= e < _))
+    | Z.modulo ?a ?b => (* TODO: non-constant denominator? *)
+      let __ := match constr:(Set) with _ => requireZcstExpr b end in
+      named_pose_proof (zbsimp! (Z.mod_pos_bound a b ltac:(eapply Z.ltb_lt; exact eq_refl) : _ <= e < _))
+    | ?op ?a ?b =>
+      let Ha := rbounded a in
+      let Hb := rbounded b in
+      let a0 := match type of Ha with ?a0 <= _ < ?a1 => a0 end in
+      let a1 := match type of Ha with ?a0 <= _ < ?a1 => a1 end in
+      let b0 := match type of Hb with ?b0 <= _ < ?b1 => b0 end in
+      let b1 := match type of Hb with ?b0 <= _ < ?b1 => b1 end in
+      match op with
+      | Z.add => named_pose_proof (zbsimp! (Z__range_add a0 a a1 Ha b0 b b1 Hb : a0 + b0 <= e < a1 + b1 - 1))
+      | Z.sub => named_pose_proof (zbsimp! (Z__range_sub a0 a a1 Ha b0 b b1 Hb : a0-b1+1 <= e < a1-b0))
+      | Z.mul => named_pose_proof (zbsimp! (Z__range_mul_nonneg a0 a a1 Ha b0 b b1 Hb (Zle_bool_imp_le 0 a0 eq_refl) (Zle_bool_imp_le 0 b0 eq_refl) : _ <= e < _))
+      (* TODO: pow *)
+      (* TODO: and, or, xor, ndn *)
+      end
+    end
+  | _ =>
+    let __ := match constr:(Set) with _ => requireZcstExpr re end in
+    constr:(zbsimp! (bounded_constant e))
+  end.
+
+(** Abstract interpretation *)
+
+Module unsigned.
+
+Definition absint_eq {T} := @eq T.
+Local Infix "=~>" := absint_eq (at level 70, no associativity).
+  
+Local Notation "absint_lemma! pf" := (ltac:(
+  cbv [absint_eq] in *;
+  etransitivity; [ eapply pf | ]; cycle -1;
+    [unshelve (repeat match goal with
+      | |-context [Z.shiftr ?x (word.unsigned ?y)] => assert_fails(is_evar x||is_evar y);
+        setoid_rewrite (Z.shiftr_div_pow2 x (word.unsigned y) (proj1 (Properties.word.unsigned_range _)))
+      | |-context [Z.shiftl ?x (word.unsigned ?y)] => assert_fails(is_evar x||is_evar y);
+        setoid_rewrite (Z.shiftl_mul_pow2 x (word.unsigned y) (proj1 (Properties.word.unsigned_range _)))
+      | |-context [?x mod (2^?y)] => assert_fails(is_evar x||is_evar y);
+        rewrite (Z.mod_small x (2^y)) by shelve
+      | |-context [word.unsigned ?x] => assert_fails(is_evar x);
+        erewrite (_:word.unsigned _=_) by shelve
+      end; exact eq_refl)
+    |..];
+    (* WHY do I need [> here? *)
+    [> (repeat match goal with
+               | H: ?P |- ?G => assert_fails (has_evar P || has_evar G); rewrite H
+               end;
+        match reverse goal with H : ?e |- ?G => is_evar e; unify e G; exact H end).. ]
+  )) (at level 10, only parsing).
+
+Lemma absint_of_Z (x : Z) (Hrange : 0 <= x < 2^width) : word.unsigned (word.of_Z x) = x.
+Proof. rewrite word.unsigned_of_Z, Z.mod_small; trivial. Qed.
+Definition absint_add (x y : word.rep) ux Hx uy Hy Hbounds : word.unsigned _ =~> _ :=
+  absint_lemma! (word.unsigned_add x y).
+Definition absint_sub (x y : word.rep) ux Hx uy Hy Hbounds : word.unsigned _ =~> _ :=
+  absint_lemma! (word.unsigned_sub x y).
+Definition absint_mul (x y : word.rep) ux Hx uy Hy Hbounds : word.unsigned _ =~> _ :=
+  absint_lemma! (word.unsigned_mul x y).
+Definition absint_and (x y : word.rep) ux Hx uy Hy : word.unsigned _ =~> _ :=
+  absint_lemma! (Properties.word.unsigned_and_nowrap x y).
+Definition absint_or (x y : word.rep) ux Hx uy Hy : word.unsigned _ =~> _ :=
+  absint_lemma! (Properties.word.unsigned_or_nowrap x y).
+Definition absint_xor (x y : word.rep) ux Hx uy Hy : word.unsigned _ =~> _ :=
+  absint_lemma! (Properties.word.unsigned_xor_nowrap x y).
+Definition absint_ndn (x y : word.rep) ux Hx uy Hy : word.unsigned _ =~> _ :=
+  absint_lemma! (Properties.word.unsigned_ndn_nowrap x y).
+Definition absint_sru (x y : word.rep) ux Hx uy Hy Hshift  : word.unsigned _ =~> _ :=
+  absint_lemma! (Properties.word.unsigned_sru_nowrap x y).
+Definition absint_slu (x y : word.rep) ux Hx uy Hy Hrange Hshift : word.unsigned _ =~> _ :=
+  absint_lemma! (word.unsigned_slu x y).
+Definition absint_divu (x y : word.rep) ux Hx uy Hy Hnz  : word.unsigned _ =~> _ :=
+  absint_lemma! (Properties.word.unsigned_divu_nowrap x y).
+Definition absint_modu (x y : word.rep) ux Hx uy Hy Hnz  : word.unsigned _ =~> _ :=
+  absint_lemma! (Properties.word.unsigned_modu_nowrap x y).
+
+Ltac named_pose_asfresh_or_id x n :=
+  let y := match constr:(Set) with _ => named_pose_asfresh x n | _ => x end in
+  y.
+
+Definition absint_eq_refl {T} v := ((@eq_refl T v) : @absint_eq T v v).
+Ltac zify_expr e :=
+  let re := rdelta e in
+  lazymatch type of e with
+  | @word.rep ?width ?word_parameters =>
+    match re with
+    | _ => match goal with H: word.unsigned e =~> _ |- _ => H end
+    | word.of_Z ?a =>
+      let Ba := rbounded a in
+      named_pose_proof (absint_of_Z a (boundscheck (X0:=0) (X1:=2^width) Ba (eq_refl true)) : @absint_eq Z (@word.unsigned _ word_parameters e) a)
+    | ?op ?a ?b =>
+      let Ha := zify_expr a in let Ra := lazymatch type of Ha with _ =~> ?x => x end in
+      let Hb := zify_expr b in let Rb := lazymatch type of Hb with _ =~> ?x => x end in
+      match op with
+      | word.and =>
+        named_pose_proof constr:(absint_and a b Ra Ha Rb Hb : @absint_eq Z (@word.unsigned _ word_parameters e) (Z.land Ra Rb))
+      | word.or =>
+        named_pose_proof constr:(absint_or a b Ra Ha Rb Hb : @absint_eq Z (@word.unsigned _ word_parameters e) (Z.lor Ra Rb))
+      | word.xor =>
+        named_pose_proof constr:(absint_xor a b Ra Ha Rb Hb : @absint_eq Z (@word.unsigned _ word_parameters e) (Z.lxor Ra Rb))
+      | word.ndn =>
+        named_pose_proof constr:(absint_ndn a b Ra Ha Rb Hb : @absint_eq Z (@word.unsigned _ word_parameters e) (Z.ldiff Ra Rb))
+
+      | word.add =>
+        let Re := named_pose_asfresh_or_id constr:(Ra+Rb) e in
+        let Be := rbounded Re in
+        let Hbounds := match type of Be with ?x0 <= ?x < ?x1 =>
+                         constr:(@boundscheck x0 x x1 Be 0 (2^width) (@eq_refl bool true)) end in
+        named_pose_proof constr:(absint_add a b Ra Ha Rb Hb Hbounds : @absint_eq Z (@word.unsigned _ word_parameters e) Re)
+      | word.sub =>
+        let Re := named_pose_asfresh_or_id constr:(Ra-Rb) e in
+        let Be := rbounded Re in
+        let Hbounds := match type of Be with ?x0 <= ?x < ?x1 =>
+                         constr:(@boundscheck x0 x x1 Be 0 (2^width) (@eq_refl bool true)) end in
+        named_pose_proof constr:(absint_sub a b Ra Ha Rb Hb Hbounds : @absint_eq Z (@word.unsigned _ word_parameters e) Re)
+      | word.mul =>
+        let Re := named_pose_asfresh_or_id constr:(Ra*Rb) e in
+        let Be := rbounded Re in
+        let Hbounds := match type of Be with ?x0 <= ?x < ?x1 =>
+                         constr:(@boundscheck x0 x x1 Be 0 (2^width) (@eq_refl bool true)) end in
+        named_pose_proof constr:(absint_mul a b Ra Ha Rb Hb Hbounds : @absint_eq Z (@word.unsigned _ word_parameters e) Re)
+
+      | word.sru =>
+        let Re := named_pose_asfresh_or_id constr:((Ra / 2^Rb)) e in
+        let Bb := rbounded Rb in
+        let pf := constr:(absint_sru a b Ra Ha Rb Hb (@boundscheck_lt _ Rb _ Bb width eq_refl): @absint_eq Z (@word.unsigned _ word_parameters e) Re) in
+        named_pose_proof pf
+      | word.slu =>
+        let Re := named_pose_asfresh_or_id constr:((Ra * 2^Rb)) e in
+        let Bb := rbounded Rb in
+        let Be := rbounded Re in
+        named_pose_proof (absint_slu a b Ra Ha Rb Hb (boundscheck (X0:=0) (X1:=2^width) Be (eq_refl true)) (@boundscheck_lt _ Rb _ Bb width eq_refl): @absint_eq Z (@word.unsigned _ word_parameters e) Re)
+      | _ => (* unknown binop or bad bounds, don't backtrack to keep Ha and Hb *)
+        constr:(@absint_eq_refl Z (@word.unsigned _ word_parameters e))
+       (* TODO: divu, modu (how do we prove denominator nonzero?) *)
+      end
+    | _ =>
+      constr:(@absint_eq_refl Z (@word.unsigned _ word_parameters e))
+    end
+  | Z =>
+    match e with
+    | _ => match goal with H: e =~> _ |- _ => H end
+    | word.unsigned ?a => zify_expr a
+    | _ => constr:(@absint_eq_refl Z e)
+    end
+  end.
+End unsigned.
